internal/examples/semantics/interfaces.go
@@ -2,72 +2,30 @@ package semantics
 
 import "fmt"
 
-type greeting interface {
-	intro() string
+// Interface with method set
+type testInterface interface {
+	Square() uint64
 }
 
-type food interface {
-	dish() string
+// Empty interface
+type emptyInterface interface{}
+
+func useInterface(t testInterface) {
+	fmt.Printf("%T", t.Square())
 }
 
-type person struct {
-	name string
-	meal string
+type TestStruct struct {
+	Number uint64
 }
 
-type animal struct {
-	bark   string
-	kibble string
+func (t TestStruct) Square() uint64 {
+	return t.Number * t.Number
 }
 
-func (p person) intro() string {
-	return p.name
-}
-
-func (a animal) intro() string {
-	return a.bark
-}
-
-func (p person) feed() string {
-	return p.meal
-}
-
-func (a animal) feed() string {
-	return a.kibble
-}
-
-func greet(g greeting) {
-	fmt.Printf("%s\n", g.intro())
-}
-
-func eating(f food) {
-	fmt.Printf("%s\n", g.dish())
-}
-
-func main() {
-	greeting(person{name: "Bob"})
-	food(animal{kibble: "Buster's Feed"})
-
-	// Empty interface
-
-	var x interface{}
-
-	// Type assertion
-
-	var y interface{} = "foo"
-
-	var s string = y.(string)
-
-	// Type switch
-
-	switch v := y.(type) {
-	case nil:
-		fmt.Println("y is nil")
-	case int:
-		fmt.Println("y is", v)
-	case bool, string:
-		fmt.Println("y is bool or string")
-	default:
-		fmt.Println("type unknown")
+func test() {
+	s := TestStruct{
+		Number: 2,
 	}
+
+	fmt.Println(s.Square())
 }
